% Exercise 3.1-5

\begin{proof}
    \begin{itemize}
        \item[$(\Rightarrow)$] Suppose $f(n) = \Theta(g(n))$, then we have 
            $0 \leq c_1 g(n) \leq f(n) \leq c_2 g(n)$ for all $n \geq n_0$, 
            where $c_1, c_2 \in \mathbb{R}^+, n, n_0 \in \mathbb{N}$.

            But then it follows that $0 \leq f(n) \leq c_2 g(n)$ for all $n \geq n_0$, 
            so $f(n) = O(g(n))$, and $0 \leq c_1 g(n) \leq f(n)$ for all $n \geq n_0$, 
            so $f(n) = \Omega(g(n))$.

        \item[$(\Leftarrow)$] 
            Now, suppose $f(n) = O(g(n))$, i.e., $0 \leq f(n) \leq c_2 g(n)$ for all 
            $n \geq n_0$ and $f(n) = \Omega(g(n))$, i.e., $0 \leq c_1 g(n) \leq f(n)$ 
            for all $n \geq n_0$, where $c_1, c_2 \in \mathbb{R}^+, n, n_0 \in \mathbb{N}$. 
            But then we have $0 \leq c_1 g(n) \leq f(n) \leq c_2 g(n)$ for all $n \geq n_0$, 
            so that $f(n) = \Theta(g(n))$.
    \end{itemize}
\end{proof}
