% Exercise 3.2-3

\begin{proof}
    Since $n! \leq n^n$ for all $n \geq 1$, we have $\lg{(n!)} \leq \lg{n^n} = n\lg{n}$
    for all $n \geq 1$, so that we have $\lg{(n!)} \leq c_2 \cdot (n\lg{n})$ for 
    $n \geq n_0$ with the identifications $c_2 = 1$ and $n_0 = 1$.
    Now, from Stirling's approximation, we have
    \[
        n! = \sqrt{2\pi n} {\biggl(\frac{n}{e}\biggr)}^n 
        \biggl(1 + \Theta \biggl(\frac{1}{n}\biggr)\biggr)
        = n^{n + 1/2} \frac{\sqrt{2\pi}}{e^n}
        \biggl(1 + \Theta\biggl(\frac{1}{n}\biggr)\biggr),
    \]
    so that
    \begin{equation*}
        \begin{split}
            \lg{(n!)} &\geq \lg{n^{n + 1/2}} + \lg{\biggl(\frac{\sqrt{2\pi}}{e^n}\biggr)} \\
                      &= \biggl(n + \frac{1}{2}\biggr)\lg{n} + \lg{\sqrt{2\pi}} - n\lg{e} \\
                      &= n\lg{n} + \frac{1}{2} \lg{n} + \lg{\sqrt{2\pi}} - n\lg{e}.
        \end{split}
    \end{equation*}
    Then, $\lg{(n!)} &\geq n\lg{n}$ for
    \begin{equation*}
        \begin{split}
            \frac{1}{2}\lg{n} + \lg{\sqrt{2\pi}} - n\lg{e} &\geq 0 \\
            \Rightarrow n &\geq \frac{\lg{\sqrt{2\pi n}}}{\lg{e}} \\
            \Rightarrow n - \frac{\lg{n}}{2\lg{e}} &\geq \frac{\lg{\sqrt{2\pi}}}{\lg{e}} \\
            \Rightarrow n - \frac{1}{2}\ln{n} &\geq \ln{\sqrt{2\pi}} \\
            \Rightarrow n \geq \ln{\sqrt{2\pi n}}.
        \end{split}
    \end{equation*}
    Thus $\lg{(n!)} = \Theta(n\lg{n})$. 

    Now,
    \[
        n! = n \cdot (n-1) \cdots 3 \cdot 2 \cdot 1 < n \cdot n \cdots n \quad (n \text{ factors}),
    \]
    for all $n > 1$, so that we have
    \[
        n! = o(n \cdot n \cdots n) = o(n^n).
    \]
    Then, 
    \[
        n! = n \cdot (n-1) \cdots 3 \cdot 2 \cdot 1 > 2 \cdot 2 \cdots 2 \quad (n \text{ factors}),
    \]
    for all $n > 2$, so that we have
    \[
        n! = \omega(2 \cdot 2 \cdots 2) = \omega(2^n).
    \]
\end{proof}
