% Exercise 3.2-1

\begin{proof}
    \begin{itemize}
        \item[\textbf{a.}] Suppose $f(n)$ and $g(n)$ are monotonically increasing 
            functions, i.e., $m \leq n \Rightarrow f(m) \leq f(n)$ and
            $g(m) \leq g(n)$. Then, clearly for $m \leq n$, we have
            \[
                f(m) + g(m) \leq f(n) + g(m) \leq f(n) + g(n),
            \]
            so that $f(n) + g(n)$ is monotonically increasing.
        \item[\textbf{b.}] Since $m \leq n \Rightarrow g(m) \leq g(n)$ and 
            $f(m) \leq f(n)$, it must also be the case that 
            \[
                m \leq n \Rightarrow g(m) \leq g(n) \Rightarrow f(g(m)) \leq f(g(n)),
            \]
            so that $f(g(n))$ is a monotonically increasing function.
        \item[\textbf{c.}] Suppose further that $f(n)$ and $g(n)$ are nonnegative.
            Then 
            \[
                m \leq n \Rightarrow f(m) \leq f(n) \Rightarrow f(m) \cdot g(n) 
                \leq f(n) \cdot g(n)
            \]
            and
            \[
                m \leq n \Rightarrow g(m) \leq g(n) \Rightarrow f(n) \cdot g(m) 
                \leq f(n) \cdot g(n),
            \]
            so that we have
            \[
                m \leq n \Rightarrow f(m) \cdot g(m) \leq f(n) \cdot g(n), 
            \]
            and $f(n) \cdot g(n)$ is a monotonically increasing function.
    \end{itemize}
\end{proof}
