% Exercise A.1-4

\begin{proof}
  We have
  \begin{equation*}
    \begin{split}
      \frac{k - 1}{2^k} &= \frac{k}{2^k} - \frac{1}{2^k} \\
      &= kx^k - x^k,
    \end{split}
  \end{equation*}
  for $x = \frac{1}{2}$. Now, since $\lvert x \rvert < 1$, from \textbf{A.6}
  and \textbf{A.8}, we have
  \begin{equation*}
    \begin{split}
      \sum_{k = 0}^\infty (k - 1) / 2^k
      &= \sum_{k = 0}^\infty kx^k - \sum_{k = 0}^\infty x^k \\
      &= \frac{x}{{(1 - x)}^2} - \frac{1}{1 - x} \\
      &= \frac{x - (1 - x)}{{(1 - x)}^2} \\
      &= \frac{2x - 1}{{(1 - x)}^2} \\
      &= \frac{1 - 1}{(-\frac{1}{2})^2} \\
      &= 0.
    \end{split}
  \end{equation*}
\end{proof}
