% Exercise 2.3-3

\begin{proof}
    We have the base case for $n = 2^1$ given by 
    \[
        T(n) = T(2) = 2 = 2\log_2{2^1} = 2 \cdot 1.
    \]
    Now, we assume as our induction step that if $n = 2^k$ for $k > 1$,
    \[
        T(n) = 2T(n/2) + n = n\lg{n}.
    \]
    Then, suppose that $n = 2^{k+1}$, so that we have
    \begin{align*}
T(n) &= 2T(2^{k+1}/2) + 2^{k+1} &\, \\
             &= 2T(2^k) + 2^{k+1} &\, \\
             &= 2(2^k\lg{2^k}) + 2^{k+1} \qquad 
                 &\text{(by our induction assumption)} \\
                 &= 2^{k+1}\lg{2^k} + 2^{k+1}\lg{2} \qquad 
                 &\text{(since $\log_2{2} = 1$)} \\
                 &= 2^{k+1}\lg{2^{k+1}} \qquad 
                 &\text{(since $\log_2{a} + \log_2{b} = \log_2{ab}$)} 
    \end{align*}
    Therefore, by induction on $n = 2^k$, $T(n) = n\lg{n}$.
\end{proof}
